\begin{prob}
\label{prob:prob-6}
\addcontentsline{toc}{section}{6. Problem 6}
已知 $y_1, y_2, y_3$ 为方程 $y^3 + py + q = 0$ 的互异复数根.
令 $\alpha = e^{\frac{2\pi i}{3}} = \frac{-1 + \sqrt{-3}}{2}$.
定义 $u = y_1 + \alpha y_2 + \alpha^2 y_3$ 及
$v = y_1 + \alpha^2 y_2 + \alpha y_3$.
试用 $p, q$ 来表示 $uv, u^3 + v^3$.
\end{prob}

\begin{soln}
答案是 $\boxed{uv = -3p, u + v = -27q.}$
利用三次单位根的性质: $\alpha^3 = 1$ 和 $\alpha^2 + \alpha + 1 = 0$,
我们有
\begin{align*}
u + v     &= 2y_1 - y_2 - y_3\\
uv        &= y_1^2 +y_2^2 +y_3^2 - y_1y_2 - y_1y_3 - y_2y_3\\
u^3 + v^3 &= 2(y_1^3 + y_2^3 + y_3^3) - 3\sum_{\text{sym}}y_1^2y_2 + 12y_1y_2y_3.
\end{align*}
再利用根与系数的关系:
\[
y_1 + y_2 + y_3 = 0, \quad
y_1y_2 + y_1y_3 + y_2y_3 = p, \quad
y_1y_2y_3 = -q,
\]
即得
\[
uv = (y_1+y_2+y_3)^2 - 3(y_1y_2 + y_1y_3 + y_2y_3) = -3p.
\]
我们有
\[
u^3 + v^3 = 2(y_1 + y_2 + y_3)^3 - 9\sum_{\text{sym}}y_1^2y_2
          = -9\sum_{\text{sym}}y_1^2y_2.
\]
另一方面, 我们有
\[
0 = (y_1 + y_2 + y_3)(y_1y_2 + y_2y_3 + y_3y_1)
  = \sum_{\text{sym}}y_1^2y_2 + 3y_1y_2y_3
  \implies -9\sum_{\text{sym}}y_1^2y_2 = -27q.
\]
\end{soln}
