\begin{prob}
\label{prob:prob-5}
\addcontentsline{toc}{section}{5. Problem 5}
设 $n$ 是任意的正整数, 记
$S_n = 1^3 + 2^3 + 3^3 + \cdots + n^3$.
\begin{enumerate}[label={(\roman*)}]
  \item 证明: $S_1 = (\frac{1(1 + 1)}{2})^2$.
  \item 如果 $S_n = (\frac{n(n+1)}{2})^2$, 证明:
    $S_{n+1} = (\frac{(n+1)(n+2)}{2})^2$.
\end{enumerate}
\end{prob}

\begin{soln}
(i) $S_1 = 1 = (\frac{1(1+1)}{2})^2$.
(ii) 我们有
\begin{align*}
\left(\frac{(n+1)(n+2)}{2}\right)^2
-
\left(\frac{n(n+1)}{2}\right)^2
&=
\left(\frac{(n+1)(n+2)}{2} - \frac{n(n+1)}{2}\right)
\left(\frac{(n+1)(n+2)}{2} + \frac{n(n+1)}{2}\right) \\
&=
(n+1)^2\left(\frac{n+2}{2} - \frac{n}{2}\right)
\left(\frac{n+2}{2} + \frac{n}{2}\right) \\
&=
(n+1)^3.
\end{align*}
\end{soln}
